#問題1.19

```
T_p,q:
a←bq+aq+ap
b←bp+aq

T_p',q' = (T_p,q)^2:
a←(bp+aq)q+(bq+aq+ap)q+(bq+aq+ap)p
 =bpq+aq^2+bq^2+aq^2+apq+bpq+apq+ap^2
 =b(q^2+2pq)+a(p^2+2q^2+2pq)
 =bq'+aq'+ap'
b←(bp+aq)p+(bq+aq+ap)q
 =bp^2+apq+bq^2+aq^2+apq
 =b(p^2+q^2)+a(q^2+2pq)
 =bp'+aq'
 ```
 より
 ```
 p'=p^2+q^2
 q'=q^2+2pq
 ```

 よって手続きは
 ```scheme
(define (square x) (* x x))
(define (even? x) (= (remainder x 2) 0))

(define (fib n)
  (fib-iter 1 0 0 1 n))

(define (fib-iter a b p q count)
  (cond ((= count 0) b)
        ((even? count)
         (fib-iter a
                   b
                   (+ (square p) (square q))
                   (+ (square q) (* 2 p q))
                   (/ count 2)))
        (else
          (fib-iter (+ (* b q) (* a q) (* a p))
                    (+ (* b p) (* a q))
                    p
                    q
                    (- count 1)))))
 ```
 となる。
